\documentclass{article}
\usepackage{vem-preamble}

\title{VEM summer project}
\author{Rory Yarr}
\date{November 2023}


\begin{document}

\maketitle

\tableofcontents

% Include the introduction
%\include{introduction}

% Include chapter 1
% \include(Chapter 1)


% \section{Example}
% \input{diagram}

% $$E_1 = \begin{cases}
%     V_1 = (\frac{1}{2},\sqrt{3}) \\
%     V_2 = (\frac{3}{2},\sqrt{3}) \\
%     V_3 = (\frac{3}{2},1+\sqrt{3}) \\ 
%     V_4 = (\frac{1}{2},1+\sqrt{3}) \\
% \end{cases}
% \quad
% E_2 = \begin{cases}
%     V_1 = (\frac{1}{2},0) \\ 
%     V_2 = (\frac{3}{2},0) \\ 
%     V_3 = (2,\frac{\sqrt{3}}{2}) \\
%     V_4 = (\frac{3}{2},\sqrt{3}) \\
%     V_5 = (\frac{1}{2}, \sqrt{3}) \\ 
%     V_6 = (0, \frac{\sqrt{3}}{2}) \\
% \end{cases}$$\\

% \subsection{E$_1$}
% For $E_1$ the square the coordinates of the centriod are, $x_{E_1} = (1, \frac{1}{2}+\sqrt{3}).$ The diameter is, $ h_{E_1} = \sqrt{2}$ and the area is $|E_1| = 1$.\\

% \subsubsection{Momonial basis}
% $
% m_1^1 = \left(\cfrac{x - 1}{\sqrt{2}}\right)^{0}\left(\cfrac{y -\frac{1}{2} - \sqrt{3}}{\sqrt{2}}\right)^{0} = 1\\
% m_x^1 = \left(\cfrac{x - 1}{\sqrt{2}}\right)^{1}\left(\cfrac{y -\frac{1}{2} - \sqrt{3}}{\sqrt{2}}\right)^{0} = \cfrac{x - 1}{\sqrt{2}}\\
% m_y^1 = \left(\cfrac{x - 1}{\sqrt{2}}\right)^{0}\left(\cfrac{y -\frac{1}{2} - \sqrt{3}}{\sqrt{2}}\right)^{1} = \cfrac{y - \frac{1}{2} - \sqrt{3}}{\sqrt{2}}$\\


% \subsubsection{DOF}

% \(
% \begin{array}{ll}
% m_x^1\bigg|_{x=\frac{1}{2}} = \cfrac{\frac{1}{2} - 1}{\sqrt{2}} = -\cfrac{1}{\sqrt{2}} & \qquad m_y^1\bigg|_{y=\sqrt{3}} = \cfrac{\sqrt{3} - \frac{1}{2} - \sqrt{3}}{\sqrt{2}} = -\cfrac{1}{\sqrt{2}} \\
% m_x^1\bigg|_{x=\frac{3}{2}} = \cfrac{\frac{3}{2} - 1}{\sqrt{2}} = \cfrac{1}{\sqrt{2}} & \qquad m_y^1\bigg|_{y=\sqrt{3}+1} = \cfrac{1+\sqrt{3} - \frac{1}{2} - \sqrt{3}}{\sqrt{2}} = \cfrac{1}{\sqrt{2}}
% \end{array}
% \)

% \subsubsection{D$_1$ Matrix}
% $D_1 = \cfrac{1}{\sqrt{2}}\begin{pmatrix}
%     \sqrt{2} & -1 & -1\\
%     \sqrt{2} & 1 & -1\\
%     \sqrt{2} & 1 & 1\\
%     \sqrt{2} & -1 & 1\\
% \end{pmatrix}$

% \subsubsection{Gradient of m}
% $\nabla m_1^1 = (0,0)$\\
% $\nabla m_x^1 = (\frac{1}{\sqrt{2}},0)$ \\
% $\nabla m_y^1 = (0,\frac{1}{\sqrt{2}})$ 

% \subsubsection{Lagrangian $\mathbf{\phi}$ basis}
% $\phi_1 = \cfrac{(x_2-x)(y_4-y)}{(x_2-x_1)(y_4-y_1)}$\\
% $\phi_1 = \cfrac{(\frac{3}{2} - x)(1+\sqrt{3} + y)}{(\frac{3}{2}-\frac{1}{2})(1+\sqrt{3} - \sqrt{3})}$\\
% Note the denominator is 1 and the same is true for the rest so they can be written in the following form.\\
% $\phi_1 = (\frac{3}{2} - x)(1 + \sqrt{3} - y)$\\
% $\phi_2 = (x - \frac{1}{2})(1 + \sqrt{3} - y)$\\
% $\phi_3 = (x - \frac{1}{2} )(y - \sqrt{3})$\\
% $\phi_4 = (\frac{3}{2} - x)(y - \sqrt{3})$

% \subsubsection{$P_0\varphi_i$}
% $
% P_0\varphi_0 = \iint_E(\frac{3}{2} - x)(1+\sqrt{3}-y)dxdy \\
% \hspace*{22pt}= \int_{\frac{1}{2}}^{\frac{3}{2}}(\frac{3}{2} - x)dx \int_{\sqrt{3}}^{1+\sqrt{3}}(1+\sqrt{3}-y)dy\\
% \hspace*{22pt}= \frac{1}{4}[3x-x^2]_{\frac{1}{2}}^{\frac{3}{2}}[2(1+\sqrt{3})x - x^2]_{\sqrt{3}}^{1+\sqrt{3}}\\
% \hspace*{22pt}= \frac{1}{4}(9/2-9/4 - 3/2+1/4)(2(1+\sqrt{3})(1+\sqrt{3})\\
% \hspace*{22pt}= \frac{1}{4}(1)(1)$



% \subsubsection{Gradient of $\phi$}
% $\nabla\phi_1 = \left(-(1 + \sqrt{3} - y),  -(\frac{3}{2}-x)\right)$\\
% $\nabla\phi_2 = \left(1 + \sqrt{3} - y,-(x - \frac{1}{2})\right)$\\
% $\nabla\phi_3 = \left(y - \sqrt{3},x - \frac{1}{2}\right)$\\
% $\nabla\phi_4 = \left(-(y-\sqrt{3}),\frac{3}{2}-x\right)$\\

% \subsubsection{$(\nabla m_x,\nabla\phi)$}
% $(\nabla m_x^1,\nabla\phi_1)_{E_1} = 
% \left(\frac{1}{\sqrt{2}},0\right)\cdot\left(-(1 + \sqrt{3} - y),  -(\frac{3}{2}-x)\right) = 
% -\frac{1}{\sqrt{2}}(1 + \sqrt{3} - y)|_{y=\sqrt{3}} = 
% -\frac{1}{\sqrt{2}}$\\
% $(\nabla m_x^1,\nabla\phi_2)_{E_1} = 
% \left(\frac{1}{\sqrt{2}},0\right)\cdot\left(1 + \sqrt{3} - y),  -(x-\frac{1}{2})\right) = 
% \frac{1}{\sqrt{2}}(1 + \sqrt{3} - y)|_{y=\sqrt{3}} = 
% \frac{1}{\sqrt{2}}$\\
% $(\nabla m_x^1,\nabla\phi_3)_{E_1} = 
% \left(\frac{1}{\sqrt{2}},0\right)\cdot\left(y-\sqrt{3}, x-\frac{1}{2}\right) = 
% \frac{1}{\sqrt{2}}(y-\sqrt{3})|_{y=\sqrt{3}+1} = 
% -\frac{1}{\sqrt{2}}$\\
% $(\nabla m_x^1,\nabla\phi_3)_{E_1} = 
% \left(\frac{1}{\sqrt{2}},0\right)\cdot\left(-(y-\sqrt{3}), \frac{3}{2}-x)\right) = 
% -\frac{1}{\sqrt{2}}(y-\sqrt{3})|_{y=\sqrt{3}+1} = 
% \frac{1}{\sqrt{2}}$\\


% \subsubsection{$\mathbf{(\nabla m_y,\nabla\phi)}$}
% $(\nabla m_y^1,\nabla\phi_1)_{E_1} = 
% \left(0,\frac{1}{\sqrt{2}}\right)\cdot\left(-(1 + \sqrt{3} - y),  -(\frac{3}{2}-x)\right) = 
% -\frac{1}{\sqrt{2}}(\frac{3}{2}-x)|_{x=\frac{1}{2}} = 
% -\frac{1}{\sqrt{2}}$\\
% $(\nabla m_y^1,\nabla\phi_2)_{E_1} = 
% \left(0,\frac{1}{\sqrt{2}}\right)\cdot\left(1 + \sqrt{3} - y),  -(x-\frac{1}{2})\right) = 
% -\frac{1}{\sqrt{2}}(x - \frac{1}{2})|_{x=\frac{3}{2}} = 
% -\frac{1}{\sqrt{2}}$\\
% $(\nabla m_y^1,\nabla\phi_3)_{E_1} = 
% \left(0,\frac{1}{\sqrt{2}}\right)\cdot\left(y-\sqrt{3}, x-\frac{1}{2}\right) = 
% \frac{1}{\sqrt{2}}(x-\frac{1}{2})|_{x=\frac{3}{2}} = 
% \frac{1}{\sqrt{2}}$\\
% $(\nabla m_y^1,\nabla\phi_3)_{E_1} = 
% \left(0,\frac{1}{\sqrt{2}}\right)\cdot\left(-(y-\sqrt{3}), \frac{3}{2}-x)\right) = 
% \frac{1}{\sqrt{2}}(\frac{3}{2}-x)|_{x=\frac{1}{2}} = 
% \frac{1}{\sqrt{2}}$\\

% \subsubsection{B$_1$ Matrix}
% $B_1 = \frac{1}{4}\begin{pmatrix}
%     1 & 1 & 1 & 1 \\
%     -d & 1 & -1 & 1\\
%     -1 & -1 & 1 & 1 
% \end{pmatrix}$

% \subsubsection{G Matrix}
% $G_1 = \begin{pmatrix}
%     1
% \end{pmatrix}
% $

% \subsection{E$_2$}
% For $E_1$ the square the coordinates of the centriod are, $x_{E_2} = (1,1).$ The diameter is, $ h_{E_1} = 2$ and the area is $|E_1| = \frac{3\sqrt{3}}{2}$.\\
% \\
% For $m_1^2 = \left(\cfrac{x - 1}{2}\right)^{0}\left(\cfrac{y - 1}{2}\right)^{0} = 1$\\
% For $m_x^2 = \left(\cfrac{x - 1}{2}\right)^{1}\left(\cfrac{y - 1}{2}\right)^{0} = \cfrac{(x-1)}{2}$\\
% For $m_y^2 = \left(\cfrac{x - 1}{2}\right)^{0}\left(\cfrac{y - 1}{2}\right)^{1} = \cfrac{y-1}{2}$\\

% \subsubsection{Monimals}
% $\begin{array}{ll}
% m_x^2|_{x=0}\hspace{1.5pt} = \cfrac{0-1}{2} = -\frac{1}{2} &\qquad m_y^2|_{y=0} \hspace{7pt}= \cfrac{0-1}{2} = -\frac{1}{2} \\
% m_x^2|_{x=\frac{1}{2}} = \cfrac{\frac{1}{2}-1}{2} = -\frac{1}{4} &\qquad m_y^2|_{y=\frac{\sqrt{3}}{2}} = \cfrac{\frac{\sqrt{3}}{2}-1}{2} = \frac{\sqrt{3}-2}{4} \\
% m_x^2|_{x=\frac{3}{2}} = \cfrac{\frac{3}{2}-1}{2} = \frac{1}{4} &\qquad m_y^2|_{y=\sqrt{3}}\, = \cfrac{\sqrt{3}-1}{2} = \frac{\sqrt{3}-1}{2} \\
% m_x^2|_{x=2}\hspace{1.5pt} = \cfrac{2-1}{2} = \frac{1}{2} &
% \end{array}$

% $D_2 = \cfrac{1}{4}\begin{pmatrix}
%     4 & -1 & - 2\\
%     4 & 1 & - 2\\
%     4 & 2 & \sqrt{3} - 2\\
%     4 & 1 & 2\sqrt{3} - 2\\
%     4 & -1 & 2\sqrt{2} - 2\\
%     4 & -2 & \sqrt{3} - 2\\
% \end{pmatrix}$

% \subsection{B matrix}
% $\nabla m_1^2 = (0,0)$\\
% $\nabla m_x^2 = (\frac{1}{2},0)$ \\
% $\nabla m_y^2 = (0,\frac{1}{2})$ \\

% Hence, \\
% $P_0m_1 = \int_E\frac{1}{E}$

\subsection{Mesh example.}
The mesh is defined using 3 sets, Vertices, Elements and Boundary. The first is an array of coordinates for each node. The Vertices element set contains a vector for each element. With the index for each node in the element labeled anti-clockwise. The boundary is a vector containing the indices in an anticlockwise order.



% Include the appendix
%\include{appendix}

\end{document}
